fixing the universe problems (fingers crossed)
- there is no denotation function denoting expressions
  into typ0 because it seems to require unlifting which
  Coq does not permit.

theories/Poly/ExprCore.v
@@ -4,6 +4,7 @@ Require Import ExtLib.Core.RelDec.
 Require Import ExtLib.Data.Fun.
 Require Import ExtLib.Data.Nat.
 Require Import ExtLib.Data.HList.
+Require Import ExtLib.Structures.Functor.
 Require Import MirrorCore.Poly.TypeI.
 Require Import MirrorCore.Poly.Ctx.
 Require Import MirrorCore.Poly.ML.
@@ -11,33 +12,12 @@ Require Import MirrorCore.Poly.ML.
 Set Implicit Arguments.
 Set Strict Implicit.
 
-(** TODO: Move this, or consolidate it! **)
-Section nth_mem.
-  Variable T : Type.
-
-  Fixpoint nth_mem (ls : list T) (n : nat) {struct ls} :
-    option { x : T & member x ls } :=
-    match ls as ls return (option { x : T & member x ls }) with
-      | nil => None
-      | l' :: ls =>
-        match n with
-          | 0 =>
-            Some (@existT _ _ l' (MZ l' ls))
-          | S n =>
-            match nth_mem ls n with
-              | Some m => Some (@existT _ _ (projT1 m) (MN l' (projT2 m)))
-              | None => None
-            end
-        end
-    end.
-End nth_mem.
-
 Module Ext : MLExt.
   Definition ext : Type := unit.
-  Definition kindof_ext (e : ext) : option kind :=
-    Some kTy.
+  Definition kindof_ext (e : ext) : option kind0 :=
+    Some kTy0.
   Definition extD (e : ext) : match kindof_ext e with
-                                | Some k => kindD k
+                                | Some k => kind0D' k
                                 | None => unit
                               end :=
     match e with
@@ -51,24 +31,24 @@ End Ext.
 
 Module MLtypes := ML Ext (* ContextHList *).
 
-(** Definnition of expression extensions **)
+(** NOTE: This precludes any environments! **)
+Record SymVal : Type :=
+{ Typ : MLtypes.typ1
+; Value : match MLtypes.typD1 nil Typ kTy1 with
+            | None => Empty_set
+            | Some T => MLtypes.Ctx.eval_Ctx T (MLtypes.Ctx.Env_nil _)
+          end
+}.
+
+(** Definition of expression extensions **)
 Module Type ExprExt.
 
-  (** NOTE: This precludes any environments! **)
-  Record SymVal : Type :=
-  { Typ : MLtypes.typ
-  ; Value : match MLtypes.typD nil Typ kTy with
-              | None => Empty_set
-              | Some T => MLtypes.Ctx.eval_Ctx T (MLtypes.Ctx.Env_nil _)
-            end
-  }.
-
   Parameter ext : Type.
-  Parameter typeof_ext : ext -> option MLtypes.typ.
+  Parameter typeof_ext : ext -> option MLtypes.typ1.
   Parameter extD : forall e : ext,
                      match typeof_ext e with
                        | Some T =>
-                         match MLtypes.typD nil T kTy with
+                         match MLtypes.typD1 nil T kTy1 with
                            | None => Empty_set
                            | Some T => MLtypes.Ctx.eval_Ctx T (MLtypes.Ctx.Env_nil _)
                          end
@@ -82,39 +62,40 @@ Module Expr (EExt : ExprExt).
 
   Inductive expr : Type :=
   | eApp  : expr -> expr -> expr
-  | eAbs  : typ -> expr -> expr
+  | eAbs  : typ0 -> expr -> expr
   | eVar  : nat -> expr
-  | eTApp : expr -> typ -> expr
+  | eTApp : expr -> typ0 -> expr
   | eExt  : EExt.ext -> expr.
 
   Section typeof_expr.
-    Variable ks : list kind.
-    Fixpoint typeof_expr  (tvs : list typ) (e : expr) : option typ.
+    Variable ks : list kind0.
+
+    Fixpoint typeof_expr  (tvs : list typ0) (e : expr) : option typ1.
       refine
         match e with
           | eApp f x =>
             match typeof_expr tvs f
-                  , typeof_expr tvs x
+                , typeof_expr tvs x
             with
-              | Some (tArr d r) , Some d' =>
-                if typ_eq d d' then Some r else None
+              | Some (tLift (tArr d r)) , Some (tLift d') =>
+                if typ0_eq d d' then Some (tLift r) else None
               | _ , _ => None
             end
           | eAbs t e =>
             match typeof_expr (cons t tvs) e with
-              | Some r => Some (tArr t r)
+              | Some (tLift r) => Some (tLift (tArr t r))
               | _ => None
             end
-          | eVar v => List.nth_error tvs v
+          | eVar v => fmap tLift (List.nth_error tvs v)
           | eTApp e t =>
             match typeof_expr tvs e with
               | Some t'' =>
                 match t'' with
-                  | tPi t' =>
-                    match kindof_typ ks t with
+                  | tPi k t' =>
+                    match kindof_typ0 ks t with
                       | Some k'' =>
                         match k'' with
-                          | kTy => Some (typ_sub t' 0 t)
+                          | kTy0 => Some (typ1_sub t' 0 t)
                           | _ => None
                         end
                       | None => None
@@ -132,13 +113,20 @@ Module Expr (EExt : ExprExt).
     Defined.
   End typeof_expr.
 
-  (** TODO: This needs to be over an arbitrary kind environment **)
   Module Env <: ContextP.
-    Definition iT := typ.
+    Definition iT := typ0.
   End Env.
 
-  Definition typD' (ks : list kind) (ctxK : Ctx.Env skindD ks) (t : typ) :=
-    match @typD ks t kTy return Ustar with
+  Definition typD1' (ks : list kind0) (ctxK : Ctx.Env kind0D' ks) (t : typ1)
+  : U1 :=
+    match @typD1 ks t kTy1 return U1 with
+      | None => Empty_set
+      | Some T => Ctx.eval_Ctx T ctxK
+    end.
+
+  Definition typD0' (ks : list kind0) (ctxK : Ctx.Env kind0D' ks) (t : typ0)
+  : U0 :=
+    match @typD0 ks t kTy0 return U0 with
       | None => Empty_set
       | Some T => Ctx.eval_Ctx T ctxK
     end.
@@ -149,58 +137,62 @@ Module Expr (EExt : ExprExt).
   Existing Instance CtxT.Functor_Ctx.
 
   Section exprD.
-    Variable ks : list kind.
+    Variable ks : list kind0.
 
     (** These have a good phase split, but it seems useful to have
      ** the context immediately to avoid the need to repeatedly destruct the
      ** types.
      **)
-    Definition TCtx (ts : list typ) (T : Ctx.Env skindD ks -> Type) : Type :=
-      @Ctx.DCtx skindD ks (fun kenv => CtxT.Ctx (typD' kenv) ts (T kenv)).
+    Definition TCtx (ts : list typ0) (T : Ctx.Env kind0D' ks -> Type) : Type :=
+      @Ctx.DCtx kind0D' ks (fun kenv => CtxT.Ctx (typD0' kenv) ts (T kenv)).
 
-    Definition TCtxT (ts : list typ) (T : typ) :=
-      TCtx ts (fun ctx => typD' ctx T).
+    Definition TCtxT1 (ts : list typ0) (T : typ1) :=
+      TCtx ts (fun ctx => typD1' ctx T).
 
-    Definition Inj_TCtxT {ts t} (val : typD' (Ctx.Env_nil _) t)
-    : TCtxT ts t.
+    Definition TCtxT0 (ts : list typ0) (T : typ0) :=
+      TCtx ts (fun ctx => typD0' ctx T).
+
+
+    Definition Inj_TCtxT {ts t} (val : typD1' (Ctx.Env_nil _) t)
+    : TCtxT1 ts t.
       red. eapply Ctx.dpure; intro.
       eapply Applicative.pure.
-      generalize (typD_weaken nil ks t); simpl.
+      generalize (typD1_weaken nil ks t); simpl.
       revert val.
-      unfold typD'.
-      refine (match typD nil t kTy as X
+      unfold typD1'.
+      refine (match typD1 nil t kTy1 as X
                     return match X with
-                             | Some T => Ctx.eval_Ctx T (Ctx.Env_nil skindD)
+                             | Some T => Ctx.eval_Ctx T (Ctx.Env_nil kind0D')
                              | None => Empty_set
                            end ->
                            match X with
                              | Some T =>
-                               match typD ks t kTy with
+                               match typD1 ks t kTy1 with
                                  | Some T' =>
                                    Ctx.DCtx
-                                     (fun env : Ctx.Env skindD nil =>
+                                     (fun env : Ctx.Env kind0D' nil =>
                                         Ctx.eval_Ctx T env ->
                                         Ctx.DCtx
-                                          (fun env' : Ctx.Env skindD ks =>
+                                          (fun env' : Ctx.Env kind0D' ks =>
                                              Ctx.eval_Ctx T' (hlist_app env env')))
                                  | None => Empty_set
                                end
                              | None => unit
                            end ->
-                           match typD ks t kTy with
+                           match typD1 ks t kTy1 with
                              | Some T => Ctx.eval_Ctx T x
                              | None => Empty_set
                            end
               with
                 | Some c => fun X =>
-                              match typD ks t kTy as Y
+                              match typD1 ks t kTy1 as Y
                                     return match Y with
                                              | Some T' =>
                                                Ctx.DCtx
-                                                 (fun env : Ctx.Env skindD nil =>
+                                                 (fun env : Ctx.Env kind0D' nil =>
                                                     Ctx.eval_Ctx c env ->
                                                     Ctx.DCtx
-                                                      (fun env' : Ctx.Env skindD ks =>
+                                                      (fun env' : Ctx.Env kind0D' ks =>
                                                          Ctx.eval_Ctx T' (hlist_app env env')))
                                              | None => Empty_set
                                            end ->
@@ -221,14 +213,39 @@ Module Expr (EExt : ExprExt).
     Eval cbv beta iota zeta delta [ Inj_TCtxT Ctx.dpure Ctx.dap Applicative.pure Applicative.ap CtxT.Applicative_Ctx CtxT.dpure CtxT.dap ] in @Inj_TCtxT.
     **)
 
-    Definition App_TCtxT {tvs t' t} :
-      TCtxT tvs (tArr t' t) ->
-      TCtxT tvs t' ->
-      TCtxT tvs t.
+    Definition App1_TCtxT {tvs t' t} :
+      TCtxT1 tvs (tLift (tArr t' t)) ->
+      TCtxT1 tvs (tLift t') ->
+      TCtxT1 tvs (tLift t).
     Proof.
-      unfold TCtxT, TCtx. unfold typD'. simpl.
-      destruct (typD ks t' kTy).
-      { destruct (typD ks t kTy).
+      unfold TCtxT1, TCtx. unfold typD1'. simpl.
+      destruct (typD0 ks t' kTy0).
+      { destruct (typD0 ks t kTy0).
+        { intros.
+          eapply Ctx.dap. 2: eapply X.
+          eapply Ctx.dap. 2: eapply X0.
+          eapply Ctx.dpure.
+          intros.
+          eapply Applicative.ap. 2: eapply X1.
+          eapply Applicative.ap. 2: eapply X2.
+          eapply Applicative.pure.
+          refine (fun x => x). }
+        { refine (fun x _ => x). } }
+      { refine (fun f _ => Ctx.dap _ f).
+        clear.
+        eapply Ctx.dpure. intros.
+        eapply Functor.fmap. eauto with typeclass_instances. 2: eapply X.
+        refine (fun x => match x with end). }
+    Defined.
+
+    Definition App_TCtxT {tvs t' t} :
+      TCtxT0 tvs (tArr t' t) ->
+      TCtxT0 tvs t' ->
+      TCtxT0 tvs t.
+    Proof.
+      unfold TCtxT0, TCtx. unfold typD0'. simpl.
+      destruct (typD0 ks t' kTy0).
+      { destruct (typD0 ks t kTy0).
         { intros.
           eapply Ctx.dap. 2: eapply X.
           eapply Ctx.dap. 2: eapply X0.
@@ -263,6 +280,7 @@ Module Expr (EExt : ExprExt).
                                     | None => Empty_set
                                   end)).
 *)
+
 
     Lemma not_lt_false a b c (H : false = a ?[ lt ] b)
     : false = (a + c) ?[ lt ] b.
@@ -313,148 +331,206 @@ Module Expr (EExt : ExprExt).
       simpl. rewrite <- not_lt_false; auto. apply plus_comm_assoc_trans.
     Defined.
 
-    Theorem lift_typ_compose_trans
+    Theorem lift_typ0_compose_trans
     : forall t s n m,
-        lift_typ s n (lift_typ s m t) = lift_typ s (n + m) t.
+        lift_typ0 s n (lift_typ0 s m t) = lift_typ0 s (n + m) t.
     Proof.
       induction t; simpl; intros.
-      { rewrite <- IHt. reflexivity. }
       { rewrite <- IHt1. rewrite <- IHt2. reflexivity. }
       { rewrite <- IHt1. rewrite <- IHt2. reflexivity. }
       { f_equal. apply lift_typ_compose_sub. }
       { reflexivity. }
     Defined.
 
-    (** TODO: Universes! **)
-    (* Require Import MirrorCore.Iso. *)
+    Theorem lift_typ1_compose_trans
+    : forall t s n m,
+        lift_typ1 s n (lift_typ1 s m t) = lift_typ1 s (n + m) t.
+    Proof.
+      induction t; simpl; intros.
+      { rewrite <- IHt. reflexivity. }
+      { f_equal. apply lift_typ0_compose_trans. }
+    Defined.
+
+    Require Import MirrorCore.Iso.
 
     Record BigIso (A B : Type) : Type :=
     { binto : A -> B
     ; boutof : B -> A
     }.
 
-    Fixpoint same {k} : kindD k -> kindD k -> Type.
+    Definition Uhuge := Type.
+
+    Fixpoint same {k} : kind0D' k -> kind0D' k -> Uhuge.
     refine
-      match k as k return kindD k -> kindD k -> Type with
-        | kTy => fun a b => BigIso a b
-        | kArr a b => fun x y =>
+      match k as k return kind0D' k -> kind0D' k -> Uhuge with
+        | kTy0 => fun a b => BigIso a b
+        | kArr0 a b => fun x y =>
                         forall c d, @same a c d ->
                                     @same b (x c) (y d)
       end%type.
     Defined.
 
-(*
-    Lemma typD_subst k tvs t' A (H : typD tvs t' k = Some A)
+    Record BigSig2 (T : Type) (A B : T -> Uhuge) : Uhuge :=
+    { value : T
+    ; projT2_1 : A value
+    ; projT2_2 : B value
+    }.
+
+    Lemma typD0_subst tvs t' A (H : typD0 tvs t' kTy0 = Some A)
     : forall t k' tvs' B,
-        typD (tvs' ++ k :: tvs) t k' = Some B ->
-        { C : _ &
-          typD (tvs' ++ tvs) (typ_sub t (length tvs') (lift_typ 0 (length tvs') t')) k' = Some C &
-          forall ts,
-            same (Ctx.eval_Ctx C ts)
-                 (let (vs,vs') := hlist_split tvs' tvs ts in
-                  Ctx.eval_Ctx B (hlist_app vs (Hcons (l := k) (Ctx.eval_Ctx A vs') vs'))) }.
+        typD0 (tvs' ++ kTy0 :: tvs) t k' = Some B ->
+        @BigSig2 (@Ctx.DCtx kind0D' (tvs' ++ tvs)
+                            (fun _ : Ctx.Env kind0D' (tvs' ++ tvs) => kind0D' k'))
+          (fun C => typD0 (tvs' ++ tvs)
+                          (typ0_sub t (length tvs') (lift_typ0 0 (length tvs') t')) k' = Some C)
+          (fun C =>
+             forall (ts : hlist kind0D' (tvs' ++ tvs)),
+               @same k'
+                     (Ctx.eval_Ctx C ts)
+                     (let (vs,vs') := hlist_split tvs' tvs ts in
+                      let val : U0 := Ctx.eval_Ctx A vs' in
+                      Ctx.eval_Ctx B (hlist_app vs (Hcons (l := kTy0) val vs'))
+)).
     Admitted.
+
+
+    Lemma typD1_subst tvs t' A (H : typD0 tvs t' kTy0 = Some A)
+    : forall t k' tvs' B,
+        typD1 (tvs' ++ kTy0 :: tvs) t k' = Some B ->
+        @BigSig2 (@Ctx.DCtx kind0D' (tvs' ++ tvs)
+                            (fun _ : Ctx.Env kind0D' (tvs' ++ tvs) => kind1D k'))
+          (fun C => typD1 (tvs' ++ tvs)
+                          (typ1_sub t (length tvs') (lift_typ0 0 (length tvs') t')) k' = Some C)
+          (fun C =>
+             forall (ts : hlist kind0D' (tvs' ++ tvs)),
+               BigIso (Ctx.eval_Ctx C ts)
+                      (let (vs,vs') := hlist_split tvs' tvs ts in
+                       let val : U0 := Ctx.eval_Ctx A vs' in
+                       Ctx.eval_Ctx B (hlist_app vs (Hcons (l := kTy0) val vs'))
+)).
     Proof.
       induction t.
-      { simpl. destruct k'; simpl.
-        { intros. specialize (IHt kTy (kTy :: tvs')).
-          simpl in *.
-          destruct (typD (kTy :: tvs' ++ k :: tvs) t kTy).
-          { unfold Quant_Ctx in H0. unfold Ctx.Quant_Ctx in H0.
-            unfold Ctx.Quant_DCtx in H0.
-            specialize (@IHt _ eq_refl).
-            rewrite lift_typ_compose_trans. destruct IHt.
-            simpl. rewrite e. eexists. reflexivity.
-            intros.
-            unfold Quant_Ctx in *.
-            unfold Ctx.Quant_Ctx in *.
-            unfold Ctx.Quant_DCtx in *.
-            unfold Ctx.eval_Ctx in *. inversion H0. subst.
-            constructor.
-            { intros.
-              remember (hlist_split tvs' tvs ts).
-              destruct p. intro.
-              specialize (b (Hcons (l := kTy) x0 ts)).
-              simpl in b. rewrite <- Heqp in b.
-              specialize (X x0). eapply b in X. apply X. }
-            { remember (hlist_split tvs' tvs ts).
-              destruct p. intro.
-              intro. specialize (X x0). clear H0.
-              specialize (b (@Hcons _ _ kTy _ x0 ts)).
-              simpl in b. rewrite <- Heqp in b. apply b. apply X. } }
-          { exfalso. inversion H0. } }
-        { inversion 1. } }
       { simpl. intros.
-        specialize (IHt2 kTy tvs').
-        specialize (IHt1 (kArr kTy k') tvs').
-        destruct (typD (tvs' ++ k :: tvs) t2 kTy). 2: inversion H0.
-        destruct (typD (tvs' ++ k :: tvs) t1 (kArr kTy k')). 2: inversion H0.
-        specialize (IHt1 _ eq_refl).
-        specialize (IHt2 _ eq_refl).
-        destruct IHt1; destruct IHt2.
-        rewrite e. rewrite e0.
+        destruct k'.
+        specialize (IHt kTy1 (k :: tvs')).
+        simpl in *.
+        destruct (typD1 (k :: tvs' ++ kTy0 :: tvs) t kTy1); try congruence.
+        specialize (@IHt _ eq_refl).
+        unfold Quant_Ctx, Ctx.Quant_Ctx, Ctx.Quant_DCtx, Ctx.eval_Ctx in *.
+        rewrite lift_typ0_compose_trans. destruct IHt.
+        simpl. rewrite projT2_3.
         eexists. reflexivity.
-        simpl. inversion H0; clear H0; subst.
-        intro. specialize (s ts). specialize (s0 ts).
-        clear - s s0.
-        destruct (hlist_split tvs' tvs ts).
-        unfold App_Ctx. simpl. unfold Ctx.dap, Ctx.dpure.
-        admit.
-*)
+        inversion H0; clear H0; subst. (** TODO: not efficient **)
+        intros. constructor.
+        { intros.
+          remember (hlist_split tvs' tvs ts).
+          destruct p. intro. 
+          specialize (projT2_4 (@Hcons _ kind0D' k _ x ts)).
+          simpl in *. rewrite <- Heqp in *.
+          specialize (X x). eapply projT2_4 in X. apply X. }
+        { remember (hlist_split tvs' tvs ts).
+          destruct p. intro.
+          intro. specialize (X x). 
+          specialize (projT2_4 (@Hcons _ _ k _ x ts)).
+          simpl in *. rewrite <- Heqp in *. apply projT2_4. apply X. } }
+      { simpl.
+        destruct k'. admit. }
+    Admitted.
 
-    Definition TApp_TCtxT {tvs t}
-               (F : TCtxT tvs (tPi t))
-               (t' : typ) (** TODO: This must to be a good type! **)
-(*               (H : typD ks t' kTy <> None) *)
-    : TCtxT tvs (typ_sub t 0 t').
+    Definition TApp_TCtxT {tvs t k}
+               (F : TCtxT1 tvs (tPi k t))
+               (t' : typ0) (** TODO: This must to be a good type! **)
+               (H : typD0 ks t' k <> None)
+    : TCtxT1 tvs (typ1_sub t 0 t').
       red in F. red. simpl in *.
       revert F.
       eapply Ctx.dap. red. intro.
-      unfold CtxT.Ctx. unfold CtxT.DCtx. unfold typD'. simpl.
+      unfold CtxT.Ctx. unfold CtxT.DCtx. unfold typD1'.
+      intros. specialize (X env0). clear env0.
+      simpl in *. unfold Quant_Ctx, Ctx.Quant_Ctx, Ctx.Quant_DCtx in X.
     Admitted.
 
-    Definition Use_TCtxT {tvs t} (mem : member t tvs)
-    : TCtxT tvs t.
+    Definition Use0_TCtxT {tvs t} (mem : member t tvs)
+    : TCtxT0 tvs t.
       red. red.
       eapply Ctx.dap.
-      2: eapply Ctx.dpure; intros; eapply (@CtxT.Use_Ctx (typD' x) _ _ mem).
+      2: eapply Ctx.dpure; intros; eapply (@CtxT.Use_Ctx (typD0' x) _ _ mem).
       simpl.
       eapply Ctx.dpure. intro.
       refine (fun x => x).
     Defined.
 
-    Definition Env_hlist : forall d tvs ctx,
-                             @typD' ks ctx d -> CtxT.Env (typD' ctx) tvs ->
-                             CtxT.Env (typD' ctx) (d :: tvs).
+    Lemma Lift_0_1 {x tvs t}
+    : CtxT.Ctx (typD0' (ks := ks) x) tvs (typD0' x t) ->
+      CtxT.Ctx (typD0' x) tvs (typD1' x (tLift t)).
+      unfold typD0', typD1'. simpl.
+      destruct (typD0 ks t kTy0).
+      { unfold Ctx.dfmap. unfold CtxT.Ctx, CtxT.DCtx, Ctx.eval_Ctx.
+        refine (fun f e => f e). }
+      { refine (fun x => x). }
+    Defined.
+
+    Definition Use1_TCtxT {tvs t} (mem : member t tvs)
+    : TCtxT1 tvs (tLift t).
+      red. red.
+      eapply Ctx.dap.
+      2: eapply Ctx.dpure; intros; eapply (@CtxT.Use_Ctx (typD0' x) _ _ mem).
+      simpl.
+      eapply Ctx.dpure. intro.
+      apply Lift_0_1.
+    Defined.
+
+    Definition Env_hlist : forall d (tvs : list typ0) ctx,
+                             @typD0' ks ctx d -> CtxT.Env (typD0' ctx) tvs ->
+                             CtxT.Env (typD0' ctx) (d :: tvs).
       unfold CtxT.Env. do 3 intro. eapply Hcons.
     Defined.
 
-    Definition Abs_TCtxT {tvs d r}
-    : option (TCtxT (d :: tvs) r -> TCtxT tvs (tArr d r)).
-      unfold TCtxT. simpl.
+    Definition Abs1_TCtxT {tvs d r}
+    : option (TCtxT1 (d :: tvs) (tLift r) -> TCtxT1 tvs (tLift (tArr d r))).
+      unfold TCtxT1. simpl.
       generalize (@Env_hlist d tvs).
-      unfold typD'.
+      unfold typD1', typD0'.
       simpl.
-      destruct (typD ks d kTy).
-      { destruct (typD ks r kTy).
+      destruct (typD0 ks d kTy0).
+      { destruct (typD0 ks r kTy0).
+        { intro. apply Some.
+          eapply Ctx.dap. eapply Ctx.dpure. intro.
+          unfold CtxT.Ctx, CtxT.DCtx, Arr0_Ctx.
+          simpl. unfold Ctx.dap, Ctx.dpure, Ctx.dfmap.
+          specialize (X x).
+          revert X. unfold Ctx.eval_Ctx.
+          auto. }
+        { exact (fun _ => None). } }
+      { exact (fun _ => None). }
+    Defined.
+
+    Definition Abs_TCtxT {tvs d r}
+    : option (TCtxT0 (d :: tvs) r -> TCtxT0 tvs (tArr d r)).
+      unfold TCtxT0. simpl.
+      generalize (@Env_hlist d tvs).
+      unfold typD0'.
+      simpl.
+      destruct (typD0 ks d kTy0).
+      { destruct (typD0 ks r kTy0).
         { intro. apply Some.
           eapply Ctx.dap. eapply Ctx.dpure. intro.
           unfold CtxT.Ctx. unfold CtxT.DCtx.
-          unfold Arr_Ctx. simpl. unfold Ctx.dap, Ctx.dpure.
+          unfold Arr0_Ctx. simpl. unfold Ctx.dap, Ctx.dpure.
           specialize (X x).
           revert X. unfold Ctx.eval_Ctx. auto. }
         { exact (fun _ => None). } }
       { exact (fun _ => None). }
     Defined.
 
-    Fixpoint exprD (tvs : list typ) (e : expr) (t : typ) {struct e}
-    : option (TCtxT tvs t).
+    Fixpoint exprD (tvs : list typ0) (e : expr) (t : typ1) {struct e}
+    : option (TCtxT1 tvs t).
       refine
         match e with
           | eExt x =>
             match EExt.typeof_ext x as toe
                   return match toe with
-                           | Some T => match typD nil T kTy with
+                           | Some T => match typD1 nil T kTy1 with
                                          | Some T => Ctx.eval_Ctx T (Ctx.Env_nil _)
                                          | None => Empty_set
                                        end
@@ -462,10 +538,10 @@ Module Expr (EExt : ExprExt).
                          end -> _
             with
               | Some t' =>
-                match typ_eq t' t with
+                match typ1_eq t' t with
                   | Some pf => fun val =>
                                  Some (match pf in _ = z
-                                             return TCtxT tvs z
+                                             return TCtxT1 tvs z
                                        with
                                          | eq_refl => Inj_TCtxT val
                                        end)
@@ -474,28 +550,34 @@ Module Expr (EExt : ExprExt).
               | None => fun _ => None
             end (EExt.extD x)
           | eApp f x =>
-            match typeof_expr ks tvs x with
-              | Some t' =>
-                match exprD tvs f (tArr t' t) with
-                  | Some f =>
-                    match exprD tvs x t' with
-                      | Some x => Some (App_TCtxT f x)
+            match t as t return option (TCtxT1 tvs t) with
+              | tLift t =>
+                match typeof_expr ks tvs x with
+                  | Some (tLift t') =>
+                    match exprD tvs f (tLift (tArr t' t)) with
+                      | Some f =>
+                        match exprD tvs x (tLift t') with
+                          | Some x => Some (App1_TCtxT f x)
+                          | None => None
+                        end
                       | None => None
                     end
-                  | None => None
+                  | _ => None
                 end
-              | None => None
+              | _ => None
             end
           | eAbs t' e =>
-            match t as t return option (TCtxT tvs t) with
-              | tArr d r =>
-                match typ_eq t' d with
+            match t as t return option (TCtxT1 tvs t) with
+              | tLift (tArr d r) =>
+                match typ0_eq t' d with
                   | Some pf =>
-                    match exprD (t' :: tvs) e r with
+                    match exprD (t' :: tvs) e (tLift r) with
                       | Some val =>
-                        match @Abs_TCtxT tvs t' r with
+                        match @Abs1_TCtxT tvs t' r with
                           | Some abs =>
-                            Some (match pf in _ = z return TCtxT tvs (tArr z r) with
+                            Some (match pf in _ = z
+                                        return TCtxT1 tvs (tLift (tArr z r))
+                                  with
                                     | eq_refl => abs val
                                   end)
                           | None => None
@@ -507,56 +589,66 @@ Module Expr (EExt : ExprExt).
               | _ => None
             end
           | eVar v =>
-            match nth_mem tvs v with
-              | Some (existT t' m) =>
-                match typ_eq t' t with
-                  | Some pf =>
-                    Some match pf in _ = z return TCtxT tvs z with
-                           | eq_refl =>
-                             Use_TCtxT m
-                         end
+            match t as t return option (TCtxT1 tvs t) with
+              | tLift t =>
+                match nth_mem tvs v with
+                  | Some (existT t' m) =>
+                    match typ0_eq t' t with
+                      | Some pf =>
+                        Some match pf in _ = z return TCtxT1 tvs (tLift z) with
+                               | eq_refl => Use1_TCtxT m
+                             end
+                      | None => None
+                    end
                   | None => None
                 end
-              | None => None
+              | _ => None
             end
           | eTApp e t' =>
             match typeof_expr ks tvs e with
               | Some t''' =>
                 match t''' with
-                  | tPi t'' =>
-                    match exprD tvs e (tPi t'') with
-                      | Some L =>
-                        match typ_eq (typ_sub t'' 0 t') t with
-                          | Some pf =>
-                            Some match pf in _ = z return TCtxT tvs z with
-                                   | eq_refl => TApp_TCtxT L _
-                                 end
-                          | None => None
+                  | tPi k t'' =>
+                    match typD0 ks t' k as Z return typD0 ks t' k = Z -> _ with
+                      | Some _ => fun pf' =>
+                        match exprD tvs e (tPi k t'') with
+                          | Some L =>
+                            match typ1_eq (typ1_sub t'' 0 t') t with
+                              | Some pf =>
+                                Some match pf in _ = z return TCtxT1 tvs z with
+                                       | eq_refl => TApp_TCtxT L _ _
+                                     end
+                              | None => None
 
+                            end
+                          | None => None
                         end
-                      | None => None
-                    end
+                      | _ => fun _ => None
+                    end eq_refl
                   | _ => None
                 end
-              | _ => None
+              | None => None
             end
         end.
+      clear - pf'. abstract congruence. (** This is a proof of False! **)
     Defined.
   End exprD.
 
   (** Some simple examples **)
   Time Eval compute in
-      match exprD (kTy :: nil) nil (eAbs (tVar 0) (eVar 0)) (tArr (tVar 0) (tVar 0)) with
+      match exprD (kTy0 :: nil) nil (eAbs (tVar 0) (eVar 0)) (tLift (tArr (tVar 0) (tVar 0))) with
         | None => (fun x => x + 1)
-        | Some val => val (@Hcons _ skindD kTy _ nat Hnil) Hnil
+        | Some val => val (@Hcons _ kind0D' kTy0 _ nat Hnil) Hnil
       end.
 
   Time Eval compute in
-      match exprD (kTy :: nil) (tVar 0 :: nil) (eApp (eAbs (tVar 0) (eVar 0)) (eVar 0)) (tVar 0) with
+      match exprD (kTy0 :: nil) (tVar 0 :: nil)
+                   (eApp (eAbs (tVar 0) (eVar 0)) (eVar 0))
+                   (tLift (tVar 0)) with
         | None => 9
         | Some val =>
-          let Ks := @Hcons _ skindD kTy _ nat Hnil in
-          val Ks (@Hcons _ (typD' Ks) (tVar 0) _ 0 Hnil)
+          let Ks := @Hcons _ kind0D' kTy0 _ nat Hnil in
+          val Ks (@Hcons _ (typD0' Ks) (tVar 0) _ 0 Hnil)
       end.
 
 End Expr.
