theories/Poly/ML.v
@@ -9,29 +9,56 @@ Require Import MirrorCore.Poly.Ctx.
 Set Implicit Arguments.
 Set Strict Implicit.
 
+(** TODO: Move this! **)
+Section nth_mem.
+  Variable T : Type.
+
+  Fixpoint nth_mem (ls : list T) (n : nat) {struct ls} :
+    option { x : T & member x ls } :=
+    match ls as ls return (option { x : T & member x ls }) with
+      | nil => None
+      | l' :: ls =>
+        match n with
+          | 0 =>
+            Some (@existT _ _ l' (MZ l' ls))
+          | S n =>
+            match nth_mem ls n with
+              | Some m => Some (@existT _ _ (projT1 m) (MN l' (projT2 m)))
+              | None => None
+            end
+        end
+    end.
+End nth_mem.
+
 (** ML-style polymorphism **)
 Definition UU := Type.
-Definition Ustar : UU := Type.
-Definition Usmall : Ustar := Type.
+Definition U1 : UU := Type.
+Definition U0 : U1 := Type.
 
-Inductive kind :=
-| kTy : kind
-| kArr : kind -> kind -> kind.
+Inductive kind1 := kTy1.
 
-Fixpoint kindD (k : kind) : UU :=
+Definition kind1D (_ : kind1) : UU :=
+  U1.
+
+Inductive kind0 :=
+| kTy0 : kind0
+| kArr0 : kind0 -> kind0 -> kind0.
+
+Fixpoint kind0D (k : kind0) (b : kind1) : kind1D b :=
   match k with
-    | kTy => Ustar
-    | kArr k1 k2 => kindD k1 -> kindD k2
+    | kTy0 => U0
+    | kArr0 k1 k2 => kind0D k1 b -> kind0D k2 b
   end.
+Definition kind0D' (k : kind0) : U1 := kind0D k kTy1.
 
-Fixpoint kind_eq (k1 k2 : kind) : option (k1 = k2) :=
+Fixpoint kind0_eq (k1 k2 : kind0) : option (k1 = k2) :=
   match k1 as k1 , k2 as k2 return option (k1 = k2) with
-    | kTy , kTy => Some eq_refl
-    | kArr l1 l2 , kArr r1 r2 =>
-      match kind_eq l1 r1 , kind_eq l2 r2 with
+    | kTy0 , kTy0 => Some eq_refl
+    | kArr0 l1 l2 , kArr0 r1 r2 =>
+      match kind0_eq l1 r1 , kind0_eq l2 r2 with
         | Some pf1 , Some pf2 =>
           Some match pf1 in _ = l , pf2 in _ = r
-                     return (kArr l1 l2 = kArr l r) with
+                     return (kArr0 l1 l2 = kArr0 l r) with
                  | eq_refl , eq_refl => eq_refl
                end
         | _ , _ => None
@@ -39,32 +66,31 @@ Fixpoint kind_eq (k1 k2 : kind) : option (k1 = k2) :=
     | _ , _ => None
   end.
 
+Fixpoint kind1_eq (k1 k2 : kind1) : option (k1 = k2) :=
+  Some match k1 as k1 , k2 as k2 return k1 = k2 with
+         | kTy1 , kTy1 => eq_refl
+       end.
+
+(*
 Record TypeCtor : Type :=
-{ Kind : kind
-; Value : kindD Kind
+{ Kind : kind0
+; Value : kind0D Kind kTy1
 }.
+*)
 
 Module Type MLExt.
   Parameter ext : Type.
-  Parameter kindof_ext : ext -> option kind.
+  Parameter kindof_ext : ext -> option kind0.
   Parameter extD : forall e : ext, match kindof_ext e with
                                      | None => unit
-                                     | Some k => kindD k
+                                     | Some k => kind0D k kTy1
                                    end.
   Parameter ext_eq : forall a b : ext, option (a = b).
 End MLExt.
 
 Module ML (Ext : MLExt) (* (MkCtx : ContextBuilder) *).
-  Definition skind := kind.
-
-  Fixpoint skindD (k : skind) : Ustar :=
-    match k with
-      | kTy => Usmall
-      | kArr k1 k2 => skindD k1 -> skindD k2
-    end.
-
   Module CtxP_skind <: ContextP.
-    Definition iT := skind.
+    Definition iT := kind0.
   End CtxP_skind.
 
   Module Ctx := ContextHList CtxP_skind.
@@ -72,74 +98,84 @@ Module ML (Ext : MLExt) (* (MkCtx : ContextBuilder) *).
   Existing Instance Ctx.Applicative_Ctx.
   Existing Instance Ctx.Functor_Ctx.
 
-  Definition skindD_to_kindD (k : kind) : option (skindD k -> kindD k) :=
-    match k as k return option (skindD k -> kindD k) with
-      | kTy => Some (fun x : Usmall => x : Ustar)
-      | _ => None
-    end.
+  Inductive typ0 :=
+  | tApp : typ0 -> typ0 -> typ0
+  | tArr : typ0 -> typ0 -> typ0
+  | tVar : nat -> typ0
+  | tExt : Ext.ext -> typ0.
 
-  Inductive typ :=
-  | tPi  : typ -> typ
-  | tApp : typ -> typ -> typ
-  | tArr : typ -> typ -> typ
-  | tVar : nat -> typ
-  | tExt : Ext.ext -> typ.
+  Inductive typ1 :=
+  | tPi : kind0 -> typ1 -> typ1
+  | tLift : typ0 -> typ1
+(*  | tArr1 : typ1 -> typ1 -> typ1 -- needed for non-type schemes *)
+  .
 
-  Fixpoint kindof_typ (ss : list kind) (t : typ) : option kind :=
+  Fixpoint kindof_typ0 (ss : list kind0) (t : typ0) : option kind0 :=
     match t with
       | tExt e => Ext.kindof_ext e
-      | tApp l r => match kindof_typ ss r
-                           , kindof_typ ss l
+      | tApp l r => match kindof_typ0 ss r
+                        , kindof_typ0 ss l
                      with
-                       | Some r , Some (kArr ld lr) =>
-                         if kind_eq ld r then Some lr else None
+                       | Some r , Some (kArr0 ld lr) =>
+                         if kind0_eq ld r then Some lr else None
                        | _ , _ => None
                      end
-      | tPi t => match kindof_typ (kTy :: ss) t with
-                   | Some kTy => Some kTy
-                   | _ => None
-                 end
-      | tArr t1 t2 => match kindof_typ ss t1
-                          , kindof_typ ss t2
+      | tArr t1 t2 => match kindof_typ0 ss t1
+                          , kindof_typ0 ss t2
                       with
-                        | Some kTy , Some kTy => Some kTy
+                        | Some kTy0 , Some kTy0 => Some kTy0
                         | _ , _ => None
                       end
       | tVar n => nth_error ss n
     end.
 
-  Fixpoint lift_typ (skip _by : nat) (t : typ) {struct t} : typ :=
+  Fixpoint kindof_typ1 (ss : list kind0) (t : typ1) : option kind1 :=
     match t with
-      | tExt e => tExt e
-      | tApp t1 t2 => tApp (lift_typ skip _by t1) (lift_typ skip _by t2)
-      | tPi t => tPi (lift_typ (S skip) _by t)
-      | tVar n => tVar (if n ?[ lt ] skip then n else (n + _by))
-      | tArr t1 t2 => tArr (lift_typ skip _by t1) (lift_typ skip _by t2)
+      | tLift t => match kindof_typ0 ss t with
+                     | Some kTy0 => Some kTy1
+                     | _ => None
+                   end
+      | tPi k t => match kindof_typ1 (k :: ss) t with
+                   | Some s' => Some kTy1
+                   | None => None
+                 end
     end.
 
-  Fixpoint typ_sub (s : typ) (skip : nat) (s' : typ) : typ :=
+  Fixpoint lift_typ0 (skip _by : nat) (t : typ0) {struct t} : typ0 :=
+    match t with
+      | tExt e => tExt e
+      | tApp t1 t2 => tApp (lift_typ0 skip _by t1) (lift_typ0 skip _by t2)
+      | tVar n => tVar (if n ?[ lt ] skip then n else (n + _by))
+      | tArr t1 t2 => tArr (lift_typ0 skip _by t1) (lift_typ0 skip _by t2)
+    end.
+
+  Fixpoint lift_typ1 (skip _by : nat) (t : typ1) {struct t} : typ1 :=
+    match t with
+      | tPi k t => tPi k (lift_typ1 (S skip) _by t)
+      | tLift t => tLift (lift_typ0 skip _by t)
+    end.
+
+  Fixpoint typ0_sub (s : typ0) (skip : nat) (s' : typ0) : typ0 :=
     match s with
       | tExt e => tExt e
-      | tApp t1 t2 => tApp (typ_sub t1 skip s') (typ_sub t2 skip s')
-      | tPi t => tPi (typ_sub t (S skip) (lift_typ 0 1 s'))
+      | tApp t1 t2 => tApp (typ0_sub t1 skip s') (typ0_sub t2 skip s')
       | tVar n =>
         if n ?[ eq ] skip then s'
         else if n ?[ lt ] skip then tVar n
              else tVar (pred n)
-      | tArr t1 t2 => tArr (typ_sub t1 skip s') (typ_sub t2 skip s')
+      | tArr t1 t2 => tArr (typ0_sub t1 skip s') (typ0_sub t2 skip s')
     end.
 
-  Fixpoint typ_eq (a b : typ) {struct a} : option (a = b) :=
+  Fixpoint typ1_sub (s : typ1) (skip : nat) (s' : typ0) : typ1 :=
+    match s with
+      | tPi k t => tPi k (typ1_sub t (S skip) (lift_typ0 0 1 s'))
+      | tLift t => tLift (typ0_sub t skip s')
+    end.
+
+  Fixpoint typ0_eq (a b : typ0) {struct a} : option (a = b) :=
     match a as a , b as b return option (a = b) with
-      | tPi a , tPi b =>
-        match typ_eq a b with
-          | Some pf => Some match pf in _ = t return tPi a = tPi t with
-                              | eq_refl => eq_refl
-                            end
-          | _ => None
-        end
       | tApp a1 a2 , tApp b1 b2 =>
-        match typ_eq a1 b1 , typ_eq a2 b2 with
+        match typ0_eq a1 b1 , typ0_eq a2 b2 with
           | Some pf1 , Some pf2 =>
             Some match pf1 in _ = t1 , pf2 in _ = t2
                        return tApp a1 a2 = tApp t1 t2
@@ -149,7 +185,7 @@ Module ML (Ext : MLExt) (* (MkCtx : ContextBuilder) *).
           | _ , _ => None
         end
       | tArr a1 a2 , tArr b1 b2 =>
-        match typ_eq a1 b1 , typ_eq a2 b2 with
+        match typ0_eq a1 b1 , typ0_eq a2 b2 with
           | Some pf1 , Some pf2 =>
             Some match pf1 in _ = t1 , pf2 in _ = t2
                        return tArr a1 a2 = tArr t1 t2
@@ -160,17 +196,31 @@ Module ML (Ext : MLExt) (* (MkCtx : ContextBuilder) *).
         end
       | tVar a , tVar b =>
         match nat_eq a b with
-          | Some pf => Some match pf in _ = t return tVar a = tVar t with
-                              | eq_refl => eq_refl
-                            end
+          | Some pf => Some (f_equal tVar pf)
           | None => None
         end
       | tExt a , tExt b =>
         match Ext.ext_eq a b with
-          | Some pf => Some match pf in _ = t return tExt a = tExt t with
-                              | eq_refl => eq_refl
-                            end
+          | Some pf => Some (f_equal tExt pf)
           | None => None
+        end
+      | _ , _ => None
+    end.
+
+  Fixpoint typ1_eq (a b : typ1) {struct a} : option (a = b) :=
+    match a as a , b as b return option (a = b) with
+      | tPi ka a , tPi kb b =>
+        match kind0_eq ka kb , typ1_eq a b with
+          | Some pfk , Some pf =>
+            Some match pfk in _ = k , pf in _ = t return tPi ka a = tPi k t with
+                   | eq_refl , eq_refl => eq_refl
+                 end
+          | _ , _ => None
+        end
+      | tLift a , tLift b =>
+        match typ0_eq a b with
+          | Some pf => Some (f_equal tLift pf)
+          | _ => None
         end
       | _ , _ => None
     end.
@@ -178,92 +228,75 @@ Module ML (Ext : MLExt) (* (MkCtx : ContextBuilder) *).
 
   (** Forall **)
   Definition Quant_Ctx
-  : forall (T : UU) {k : skind} {ks : list skind},
-      ((skindD k -> T) -> T) ->
-      Ctx.Ctx skindD (k :: ks) T -> Ctx.Ctx skindD ks T :=
-    @Ctx.Quant_Ctx skindD.
+  : forall (T : UU) {k : kind0} {ks : list kind0},
+      ((kind0D' k -> T) -> T) ->
+      Ctx.Ctx kind0D' (k :: ks) T -> Ctx.Ctx kind0D' ks T :=
+    @Ctx.Quant_Ctx kind0D'.
 
   (** Arrow **)
-  Definition Arr_Ctx {ks : list skind} (L R : Ctx.Ctx skindD ks (kindD kTy))
-  : Ctx.Ctx skindD ks (kindD kTy) :=
+  Definition Arr0_Ctx {ks : list kind0}
+             (L R : Ctx.Ctx kind0D' ks (kind0D' kTy0))
+  : Ctx.Ctx kind0D' ks (kind0D' kTy0) :=
     ap (ap (pure (fun l r => l -> r)) L) R.
 
   (** Application **)
-  Definition App_Ctx {ks : list skind} {k k' : kind}
-             (F : Ctx.Ctx skindD ks (kindD (kArr k' k)))
-             (X : Ctx.Ctx skindD ks (kindD k'))
-  : Ctx.Ctx skindD ks (kindD k) :=
+  Definition App_Ctx {ks : list kind0} {k k' : kind0}
+             (F : Ctx.Ctx kind0D' ks (kind0D' (kArr0 k' k)))
+             (X : Ctx.Ctx kind0D' ks (kind0D' k'))
+  : Ctx.Ctx kind0D' ks (kind0D' k) :=
     ap (ap (pure (fun f x => f x)) F) X.
 
   (** Injection **)
-  Definition Inj_Ctx {ks : list skind} (k : kind) (val : kindD k)
-  : Ctx.Ctx skindD ks (kindD k) := pure val.
+  Definition Inj_Ctx {ks : list kind0} (k : kind0) (val : kind0D' k)
+  : Ctx.Ctx kind0D' ks (kind0D' k) := pure val.
 
-  Fixpoint nth_mem_kind (ks : list skind) (k : skind) (n : nat) : option (member k ks) :=
-    match ks as ks return option (member k ks) with
-      | nil => None
-      | cons k' ks =>
-        match n with
-          | 0 => match kind_eq k' k with
-                   | Some pf => Some match pf in _ = kk return member kk (cons k' ks) with
-                                       | eq_refl => MZ _ _
-                                     end
-                   | None => None
-                 end
-          | S n => match nth_mem_kind ks k n with
-                     | Some m => Some (@MN _ _ _ _ m)
-                     | None => None
-                   end
-        end
-    end.
-
-  Fixpoint typD (ks : list skind) (t : typ) (k : kind)
-  : option (Ctx.Ctx skindD ks (kindD k)) :=
+  Fixpoint typD0 (ks : list kind0) (t : typ0) (k : kind0)
+  : option (Ctx.Ctx kind0D' ks (kind0D' k)) :=
     match t with
-      | tPi t =>
-        match k as k return option (Ctx.Ctx skindD ks (kindD k))
-        with
-          | kTy =>
-            match typD (cons kTy ks) t kTy with
-              | Some T => Some (Quant_Ctx (k := kTy) (fun P => forall x : Usmall, P x) T)
-              | _ => None
-            end
-          | _ => None
-        end
       | tArr t t' =>
-        match k as k return option (Ctx.Ctx skindD ks (kindD k))
+        match k as k return option (Ctx.Ctx kind0D' ks (kind0D' k))
         with
-          | kTy =>
-            match typD ks t kTy , typD ks t' kTy with
-              | Some K , Some T => Some (Arr_Ctx K T)
+          | kTy0 =>
+            match typD0 ks t kTy0 , typD0 ks t' kTy0 with
+              | Some K , Some T => Some (Arr0_Ctx K T)
               | _ , _ => None
             end
           | _ => None
         end
       | tApp t t' =>
-        let k' := kTy in
-        (** NOTE: This is fine since [tPi] only ranges over [*] **)
-        match typD ks t' k' , typD ks t (kArr k' k) with
-          | Some T , Some F => Some (App_Ctx F T)
-          | _ , _ => None
+        match kindof_typ0 ks t' with
+          | Some k' =>
+            match typD0 ks t' k' , typD0 ks t (kArr0 k' k) with
+              | Some T , Some F => Some (App_Ctx F T)
+              | _ , _ => None
+            end
+          | _ => None
         end
       | tVar v =>
-        match skindD_to_kindD k , nth_mem_kind ks k v with
-          | Some f , Some m => Some (@fmap _ _ _ _ f (Ctx.Use_Ctx m))
-          | _ , _ => None
+        match nth_mem ks v with
+          | Some (existT k' m) =>
+            match kind0_eq k' k with
+              | Some pf => Some match pf in _ = kk
+                                      return Ctx.Ctx kind0D' ks (kind0D' kk)
+                                with
+                                  | eq_refl => Ctx.Use_Ctx m
+                                end
+              | None => None
+            end
+          | _ => None
         end
       | tExt u =>
         match Ext.kindof_ext u as koe
               return match koe with
                        | None => unit
-                       | Some k => kindD k
+                       | Some k => kind0D' k
                      end -> _
         with
           | Some k' =>
-            match kind_eq k' k with
+            match kind0_eq k' k with
               | Some pf => fun f =>
                 Some (match pf in _ = k
-                            return kindD k' -> Ctx.Ctx skindD ks (kindD k) with
+                            return kind0D' k' -> Ctx.Ctx kind0D' ks (kind0D' k) with
                         | eq_refl => fun v => Inj_Ctx _ v
                       end f)
               | None => fun _ => None
@@ -272,19 +305,39 @@ Module ML (Ext : MLExt) (* (MkCtx : ContextBuilder) *).
         end (Ext.extD u)
     end.
 
-  Fixpoint typD_weaken ks ks' t {struct t}
-  : match typD ks t kTy , typD (ks ++ ks') t kTy return Type with
+  Fixpoint typD1 (ks : list kind0) (t : typ1) (k : kind1)
+  : option (Ctx.Ctx kind0D' ks (kind1D k)) :=
+    match t with
+      | tPi k' t =>
+        match k as k return option (Ctx.Ctx kind0D' ks (kind1D k))
+        with
+          | kTy1 =>
+            match typD1 (cons k' ks) t kTy1 with
+              | Some T =>
+                Some (Quant_Ctx (k := k')
+                                (fun P => forall x : kind0D k' kTy1, P x) T)
+              | _ => None
+            end
+        end
+      | tLift t =>
+        match k as k return option (Ctx.Ctx kind0D' ks (kind1D k)) with
+          | kTy1 =>
+            fmap (fmap (fun x : U0 => x : U1)) (typD0 ks t kTy0)
+        end
+    end.
+
+  Fixpoint typD1_weaken ks ks' t {struct t}
+  : match typD1 ks t kTy1 , typD1 (ks ++ ks') t kTy1 return Type with
       | Some T , Some T' =>
-        @Ctx.DCtx skindD ks (fun env =>
-           @Ctx.eval_Ctx skindD ks (fun _ => kindD kTy) T env ->
-           @Ctx.DCtx skindD ks' (fun env' =>
-                            @Ctx.eval_Ctx skindD (ks ++ ks') (fun _ => kindD kTy) T'
-                                          (hlist_app env env')))
+        @Ctx.DCtx kind0D' ks (fun env =>
+                                @Ctx.eval_Ctx kind0D' ks (fun _ => kind1D kTy1) T env ->
+                                @Ctx.DCtx kind0D' ks' (fun env' =>
+                                                         @Ctx.eval_Ctx kind0D' (ks ++ ks') (fun _ => kind1D kTy1) T'
+                                                                       (hlist_app env env')))
 
       | Some _ , None => Empty_set
       | None , _ => unit
     end.
-  Proof.
     (** TODO: There has got to be a cleaner statement for this **)
 (*
     destruct t; simpl.
